---
title: Abstract Algebra - Assignment 3
author: Jaan Tollander de Balsch, 452056
date: \today
header-includes: \usepackage{unicode-math}
---
This report uses definitions by [@contemporary_abstract_algebra] chapters Groups, Finite Groups, and Subgroups.


## Problem 3
Let \(G\) be a group and let \(H\) and \(K\) be subgroups of \(G\). Show that the set \(HK:=\{hÂ·kâˆ£hâˆˆH,kâˆˆK\}\) is a subgroup of \(G\) if and only if \(HK=KH.\)

---

In order to prove that \(HK\) is a subgroup of \(G\) if only if \(HK=KH\) it needs to satisfy the subgroup test. In this case, we will be using the **Two-Step Subgroup Test**. The subset \(HK\) is **nonempty** because subsets \(H\) and \(K\) are non-empty.

**Closure under operation**: For all \(a,bâˆˆHK\) implies \(aÂ·bâˆˆHK\).

1) Let \(a=h_1Â·k_1\) and \(b=h_2Â·k_2\) where \(h_1,h_2âˆˆH\) and \(k_1,k_2âˆˆK\).
2) The definition of \(HK\) implies that \(h_1Â·k_1âˆˆH\) and \(h_2Â·k_2âˆˆK\).
3) A further implication is that
\(h_1,k_1âˆˆH\) and \(h_2,k_2âˆˆK\).
4) Therefore all \(hâˆˆH\) must be in \(K\) and all \(kâˆˆK\) must be in \(H\) for \(HK\) to be a subgroup of \(G\).

**Closure under inverse**: For all \(aâˆˆHK\) implies \(a^{-1}âˆˆHK\).

1) Let \(a=hÂ·k\) where \(hâˆˆH\) and \(kâˆˆK\).
2) Then \((hÂ·k)^{-1}âˆˆHK\).
3) Equivalently \(k^{-1}Â·h^{-1}âˆˆHK\).
4) Definition of \(HK\) implies \(k^{-1}âˆˆH\) and \(h^{-1}âˆˆK\).
5) Therefore all inverses of \(hâˆˆH\) must be in \(K\) and all inverses of \(kâˆˆK\) must be in \(H\) for \(HK\) to be a subgroup of \(G\).

For \(HK\) to be a subgroup of \(G\), subgroups \(H\) and \(K\) must be equivalent, and therefore \(HK=KH\).


## Problem 4
Let \(GL_2(â„)\) denote the group of all invertible \(2Ã—2\)-matrices with real entries. Let
\[
A:=\left[\begin{matrix}1 & 1\\0 & 1\end{matrix}\right]
\text{   and   }
B:=\left[\begin{matrix}0 & -1\\1 & 0\end{matrix}\right]
\]

### (a)
Show that \(A\) and \(B\) are indeed invertible, and determine their order.

---

The inverses of \(A\) and \(B\) are
\[
A^{-1}=\left[\begin{matrix}1 & -1\\0 & 1\end{matrix}\right]
\]
and
\[
B^{-1}=\left[\begin{matrix}0 & 1\\-1 & 0\end{matrix}\right].
\]

The order of \(A\) is infinite because there does not exist a positive integer \(n\) such that \(A^n=ğˆ\)
\[
A^{n}=\left[\begin{matrix}1 & n\\0 & 1\end{matrix}\right].
\]

The sequence \(B^1,B^2,B^3,B^4\)
\[
\left ( \left[\begin{matrix}0 & -1\\1 & 0\end{matrix}\right], \quad \left[\begin{matrix}-1 & 0\\0 & -1\end{matrix}\right], \quad \left[\begin{matrix}0 & 1\\-1 & 0\end{matrix}\right], \quad \left[\begin{matrix}1 & 0\\0 & 1\end{matrix}\right]\right )
\]

The order of \(B\) is \(4\) because of \(B^4=ğˆ.\)


### (b)
Compute the product \(Aâ‹…B\) and determine its order. What is your conclusion?

---

The product \(Aâ‹…B\)
\[
Aâ‹…B=\left[\begin{matrix}1 & -1\\1 & 0\end{matrix}\right]
\]

The sequence \((Aâ‹…B)^1,(Aâ‹…B)^2â€¦,(Aâ‹…B)^6\)
\[
\left ( \left[\begin{matrix}1 & -1\\1 & 0\end{matrix}\right], \quad \left[\begin{matrix}0 & -1\\1 & -1\end{matrix}\right], \quad \left[\begin{matrix}-1 & 0\\0 & -1\end{matrix}\right], \quad \left[\begin{matrix}-1 & 1\\-1 & 0\end{matrix}\right], \quad \left[\begin{matrix}0 & 1\\-1 & 1\end{matrix}\right], \quad \left[\begin{matrix}1 & 0\\0 & 1\end{matrix}\right]\right )
\]

The order of \(Aâ‹…B\) is \(6\) because of \((Aâ‹…B)^6=ğˆ.\)

As a conclusion, the order of an element \(a\) in group \(G\) is the size the set of distinct elements generated by the powers of \(a\).


## Problem 5
Let \(a,b,\) and \(c\) be elements in a group \(G\).

### (a)
Show that \(a\) and \(a^{-1}\) have the same order.

---

Let the order of the element \(a\) be the smallest positive integer \(n\) such that
\[
\begin{aligned}
a^n &= e \\
(a^n)^{-1} &= e \\
(a^{-1})^{n} &= e.
\end{aligned}
\]
The socks-shoes property \((aÂ·b)^{-1}=b^{-1}Â·a^{-1}\) implies that \((a^n)^{-1}=(a^{-1})^n.\)

If there was a positive integer \(m < n\) such that \((a^{-1})^{m}=e\) this would imply that \(a^{m}=e\) which is a contradiction. Therefore \(n\) is also the smallest positive integer such that \((a^{-1})^n=e\). This implies that the order of \(a^{-1}\) is also \(n\). The same logic also works for sections (b) and (c).


### (b)
Show that \(b^{-1}Â·aÂ·b\) and \(a\) have the same order.

---

Let the order of the element \(b^{-1}Â·aÂ·b\) be the smallest positive integer \(n\) such that
\[
\begin{aligned}
(b^{-1}Â·aÂ·b)^n&=e \\
(b^{-1}Â·aÂ·b)Â·(b^{-1}Â·aÂ·b)Â·...Â·(b^{-1}Â·aÂ·b)&=e \\
b^{-1}Â·aÂ·(bÂ·b^{-1})Â·aÂ·(bÂ·b^{-1})Â·...Â·(bÂ·b^{-1})Â·aÂ·b&=e \\
b^{-1}Â·a^nÂ·b&=e \\
a^n&=bÂ·eÂ·b^{-1} \\
a^n&=e.
\end{aligned}
\]
This implies that the order of element \(a\) is also \(n\).


### (c)
Using (b), show that \(aÂ·b\) and \(bÂ·a\) have the same order. Deduce from this, that \(aÂ·bÂ·c\) and \(bÂ·cÂ·a\) have the same order.

---

Let the order of the element \(aÂ·b\) be the smallest positive integer \(n\) such that
\[
\begin{aligned}
(aÂ·b)^n&=e \\
aÂ·(bÂ·a)^{n-1}Â·b&=e \\
aÂ·(bÂ·a)^{n-1}&=eÂ·b^{-1} \\
aÂ·(bÂ·a)^{n-1}&=b^{-1}Â·e \\
(bÂ·a)Â·(bÂ·a)^{n-1}&=e \\
(bÂ·a)^n&=e
\end{aligned}
\]
This implies that the order of element \(bÂ·a\) is also \(n\). Using this property, we can also prove that the order of element \(aÂ·bÂ·c\) is the same as the order of element \(bÂ·cÂ·a\)
\[
\begin{aligned}
(aÂ·bÂ·c)^n&=e \\
(aÂ·b')^n&=e,â€ƒb'=bÂ·c \\
(b'Â·a)^n&=e \\
(bÂ·cÂ·a)^{n}&=e.
\end{aligned}
\]


## References
